src/ReactorModel/Execution/Trace.lean
@@ -4,17 +4,42 @@ open Classical
 
 namespace Execution
 
-inductive InstStep : State → State → Type  
-  | skip : (s.Allows rcn.id) → (¬s.Triggers rcn) → InstStep s (s.record rcn.id)
-  | exec : (s.Allows rcn.id) → (s.Triggers rcn)  → InstStep s (s.exec rcn |>.record rcn.id)
+inductive InstStep.Skip : State → State → Type  
+  | mk : (s.Allows rcn.id) → (¬s.Triggers rcn) → Skip s (s.record rcn.id)
+
+notation s₁:max " ⇓ₛ " s₂:max => InstStep.Skip s₁ s₂
+
+def InstStep.Skip.rcn : (s₁ ⇓ₛ s₂) → s₁.rtr.Valid .rcn
+  | mk (rcn := rcn) .. => rcn
+
+def InstStep.Skip.allows_rcn : (e : s₁ ⇓ₛ s₂) → s₁.Allows e.rcn
+  | mk h .. => h
+
+def InstStep.Skip.not_triggers : (e : s₁ ⇓ₛ s₂) → ¬s₁.Triggers e.rcn
+  | mk _ h => h
+
+inductive InstStep.Exec : State → State → Type  
+  | mk : (s.Allows rcn.id) → (s.Triggers rcn) → Exec s (s.exec rcn |>.record rcn.id)
+
+notation s₁:max " ⇓ₑ " s₂:max => InstStep.Exec s₁ s₂
+
+def InstStep.Exec.rcn : (s₁ ⇓ₑ s₂) → s₁.rtr.Valid .rcn
+  | mk (rcn := rcn) .. => rcn
+
+def InstStep.Exec.allows_rcn : (e : s₁ ⇓ₑ s₂) → s₁.Allows e.rcn
+  | mk h .. => h
+
+inductive InstStep (s₁ s₂ : State)
+  | skip (e : InstStep.Skip s₁ s₂)
+  | exec (e : InstStep.Exec s₁ s₂)
 
 notation s₁:max " ⇓ᵢ " s₂:max => InstStep s₁ s₂
 
 def InstStep.rcn : (s₁ ⇓ᵢ s₂) → s₁.rtr.Valid .rcn
-  | skip (rcn := rcn) .. | exec (rcn := rcn) .. => rcn
+  | skip e | exec e => e.rcn
 
 def InstStep.allows_rcn : (e : s₁ ⇓ᵢ s₂) → s₁.Allows e.rcn
-  | skip h _ | exec h _ => h
+  | skip e | exec e => e.allows_rcn
 
 -- TODO?: Once all else is settled, return this to being only transitive but not reflexive.
 --        Then you can remove the `fresh` condiction on `ClosedExecution`.
