src/ReactorModel/Objects/Reactor/Basic.lean
@@ -45,10 +45,4 @@ abbrev state (rtr : Reactor) := ReactorType.state rtr
 abbrev rcns  (rtr : Reactor) := ReactorType.rcns rtr
 abbrev nest  (rtr : Reactor) := ReactorType.nest rtr
 
-noncomputable def scheduledTags (rtr : Reactor) : Set Time.Tag := 
-  { g | ∃ i a, (rtr[.act][i] = some a) ∧ (g ∈ a.keys) }
-
-def dependencies (rtr : Reactor) (rcn : ID) : Set ID := 
-  { rcn' | rcn' <[rtr] rcn }
-
 end Reactor
