src/ReactorModel/Determinism/InstStep.lean
@@ -3,29 +3,6 @@ import ReactorModel.Determinism.Dependency
 open Classical ReactorType
 
 namespace Execution
-namespace InstStep
-
-theorem equiv : (s₁ ⇓ᵢ s₂) → s₁.rtr ≈ s₂.rtr
-  | skip .. => .refl
-  | exec .. => by simp [State.record_preserves_rtr, Equivalent.symm $ s₁.exec_equiv _]
-
-theorem deterministic (e₁ : s ⇓ᵢ s₁) (e₂ : s ⇓ᵢ s₂) (h : e₁.rcn = e₂.rcn) : s₁ = s₂ := by
-  cases e₁ <;> cases e₂ <;> 
-  all_goals 
-    simp [rcn] at h
-    subst h
-    first | rfl | contradiction
-
-theorem acyclic (e : s₁ ⇓ᵢ s₂) : e.rcn ≮[s₁.rtr] e.rcn :=
-  e.allows_rcn.acyclic
-
-theorem wellordered (e₁ : s₁ ⇓ᵢ s₂) (e₂ : s₂ ⇓ᵢ s₃) : e₂.rcn ≮[s₁.rtr] e₁.rcn :=
-  sorry
-
-end InstStep 
-
-theorem InstStep.rtr_contains_rcn (e : s₁ ⇓ᵢ s₂) : (e.rcn.id ∈ s₁.rtr[.rcn].ids) :=
-  sorry -- s₁.operation_to_contains e.wfOp 
 
 theorem InstStep.rcn_not_mem_progress (e : s₁ ⇓ᵢ s₂) : e.rcn.id ∉ s₁.progress := 
   sorry -- e.allows.unprocessed
@@ -62,18 +39,11 @@ theorem InstStep.not_mem_progress :
 
 -- Corollary of `InstStep.mem_progress`.
 theorem InstStep.monotonic_progress : (s₁ ⇓ᵢ s₂) → rcn' ∈ s₁.progress → rcn' ∈ s₂.progress := 
-  (·.mem_progress_iff.mpr $ .inr ·)
-
-theorem InstStep.strict_monotonic_progress :
-  (s₁ ⇓ᵢ s₂) → s₁.progress ⊂ s₂.progress := by
-  sorry
+  sorry -- (·.mem_progress_iff.mpr $ .inr ·)
 
 -- Corollary of `InstStep.mem_progress`.
 theorem InstStep.rcn_mem_progress : (e : s₁ ⇓ᵢ s₂) → e.rcn.id ∈ s₂.progress := 
   (·.mem_progress_iff.mpr $ .inl rfl)
-
-theorem InstStep.not_Closed (e : s₁ ⇓ᵢ s₂) : ¬s₁.Closed := by
-   sorry
 
 theorem identified_changes_equiv_changes {cs : List Change} {o : List (Identified Change)} : 
   (cs.map ({ id := i, obj := ·}) = o) → (o.map (·.obj) = cs) := by
@@ -242,10 +212,116 @@ theorem InstStep.indep_rcns_indep_output :
           exact he.eq_obj?_nest h hco hco' 
         )
     -/
-  
-theorem InstStep.progress_eq (e : s₁ ⇓ᵢ s₂) : s₂.progress = s₁.progress.insert e.rcn.id := 
+
+namespace InstStep
+
+theorem Skip.equiv : (s₁ ⇓ₛ s₂) → s₁.rtr ≈ s₂.rtr
+  | mk .. => .refl
+
+theorem Skip.progress_eq : (e : s₁ ⇓ₛ s₂) → s₂.progress = s₁.progress.insert e.rcn.id
+  | mk .. => rfl
+
+theorem Skip.progress_mono (e : s₁ ⇓ₛ s₂) : s₁.progress ⊆ s₂.progress := by
+  simp [e.progress_eq]
+  apply Set.subset_insert
+
+theorem Skip.triggers_iff (e : s₁ ⇓ₛ s₂) : (s₁.Triggers ⟨i, h₁⟩) ↔ (s₂.Triggers ⟨i, h₂⟩) := by 
+  cases e
+  case mk rcn _ _ =>
+    constructor
+    all_goals
+      intro h
+      exact h.progress_agnostic (s₁.record_preserves_rtr rcn) (s₁.record_preserves_tag rcn)
+
+theorem Skip.mem_progress_iff (e : s₁ ⇓ₛ s₂) : 
+    (rcn' ∈ s₂.progress) ↔ (rcn' = e.rcn ∨ rcn' ∈ s₁.progress) := by
   sorry
 
-theorem InstStep.prepend_indep (e₁ : s₁ ⇓ᵢ s₂) (e₂ : s₂ ⇓ᵢ s₃) (h : e₁.rcn ≮[s₁.rtr] e₂.rcn) :
+theorem Skip.preserves_allows_indep (e₁ : s₁ ⇓ₛ s₂) (e₂ : s₂ ⇓ₛ s₃) (h : e₁.rcn ≮[s₁.rtr] e₂.rcn) : 
+    s₁.Allows e₂.rcn where
+  unprocessed := Set.not_mem_subset e₁.progress_mono $ e₂.allows_rcn.unprocessed
+  deps := by
+    intro i hi
+    have h' := Reactor.equiv_eq_dependencies e₁.equiv |>.symm ▸ e₂.allows_rcn.deps
+    refine e₁.mem_progress_iff.mp (h' hi) |>.resolve_left ?_
+    intro hc; subst hc; contradiction
+
+set_option pp.proofs.withType false
+theorem Skip.swap_indep_skip (e₁ : s₁ ⇓ₛ s₂) (e₂ : s₂ ⇓ₛ s₃) (h : e₁.rcn ≮[s₁.rtr] e₂.rcn) : 
+    ∃ (s₂' : _) (f₁ : s₁ ⇓ₛ s₂') (f₂ : s₂' ⇓ₛ s₃), (f₁.rcn.id = e₂.rcn) ∧ (f₂.rcn.id = e₁.rcn) := by 
+  have ha := e₁.preserves_allows_indep e₂ h
+  have ht := e₁.triggers_iff (h₁ := sorry) |>.not.mpr e₂.not_triggers
+  have e₁' := Skip.mk ha ht
+  simp at e₁'
+  exists _, e₁'
+  sorry -- TODO: This is super annoying. Is there a better way to approach this?
+        --       Do we need more preservation theorems for `Allows` and `Triggers` first?
+
+theorem Skip.swap_indep_exec (e₁ : s₁ ⇓ₛ s₂) (e₂ : s₂ ⇓ₑ s₃) (h : e₁.rcn ≮[s₁.rtr] e₂.rcn) : 
+    ∃ (s₂' : _) (f₁ : s₁ ⇓ₑ s₂') (f₂ : s₂' ⇓ₛ s₃), (f₁.rcn.id = e₂.rcn) ∧ (f₂.rcn.id = e₁.rcn) := by 
+  sorry
+
+theorem Skip.swap_indep (e₁ : s₁ ⇓ₛ s₂) (e₂ : s₂ ⇓ᵢ s₃) (h : e₁.rcn ≮[s₁.rtr] e₂.rcn) : 
+    ∃ (s₂' : _) (f₁ : s₁ ⇓ᵢ s₂') (f₂ : s₂' ⇓ₛ s₃), (f₁.rcn.id = e₂.rcn) ∧ (f₂.rcn.id = e₁.rcn) := by 
+  cases e₂
+  case skip e₂ =>
+    have ⟨_, e₁', e₂', _⟩ := e₁.swap_indep_skip e₂ h
+    exists _, skip e₁', e₂'
+  case exec e₂ =>
+    have ⟨_, e₁', e₂', _⟩ := e₁.swap_indep_exec e₂ h
+    exists _, exec e₁', e₂'
+
+theorem Exec.equiv : (s₁ ⇓ₑ s₂) → s₁.rtr ≈ s₂.rtr
+  | mk .. => by simp [State.record_preserves_rtr, Equivalent.symm $ s₁.exec_equiv _]
+
+theorem Exec.progress_eq : (e : s₁ ⇓ₑ s₂) → s₂.progress = s₁.progress.insert e.rcn.id
+  | mk .. => rfl
+
+theorem not_Closed (e : s₁ ⇓ᵢ s₂) : ¬s₁.Closed := by
+  intro c
+  have h := c ▸ e.allows_rcn.unprocessed
+  simp [Partial.mem_ids_iff] at h 
+  have := e.rcn.obj?_id_eq_obj ▸ h e.rcn.obj
+  contradiction 
+
+theorem equiv : (s₁ ⇓ᵢ s₂) → s₁.rtr ≈ s₂.rtr
+  | skip e | exec e => e.equiv
+
+theorem deterministic (e₁ : s ⇓ᵢ s₁) (e₂ : s ⇓ᵢ s₂) (h : e₁.rcn = e₂.rcn) : s₁ = s₂ := by
+  cases e₁ <;> cases e₂
+  all_goals 
+    case _ e₁ e₂ => 
+      cases e₁; cases e₂
+      simp [rcn] at h
+      subst h
+      first | rfl | contradiction
+
+theorem acyclic (e : s₁ ⇓ᵢ s₂) : e.rcn ≮[s₁.rtr] e.rcn :=
+  e.allows_rcn.acyclic
+
+theorem progress_eq : (e : s₁ ⇓ᵢ s₂) → s₂.progress = s₁.progress.insert e.rcn.id
+  | skip e | exec e => e.progress_eq  
+
+/-
+By cases on e₁ and e₂:
+(1) skip.skip:
+    then both didn't trigger and nothing about the reactors changed, so it is easy to show that
+    switching the order preserves non-triggering.
+
+(2)&(3) exec.skip and skip.exec:
+        using `preserves_triggers` it should be easy
+
+(4) exec.exec: 
+    reduces to a theorem on State.exec?
+-/
+theorem prepend_indep (e₁ : s₁ ⇓ᵢ s₂) (e₂ : s₂ ⇓ᵢ s₃) (h : e₁.rcn ≮[s₁.rtr] e₂.rcn) :
     ∃ (s₂' : _) (e₁' : s₁ ⇓ᵢ s₂') (e₂' : s₂' ⇓ᵢ s₃), e₁'.rcn.id = e₂.rcn ∧ e₂'.rcn.id = e₁.rcn := by
-  sorry 
+  cases e₁ 
+  case skip e₁ => 
+    have ⟨_, e₁', e₂', _⟩ := e₁.swap_indep e₂ h
+    exists _, e₁', skip e₂'
+  case exec e₁ =>
+    sorry 
+
+end InstStep 
+end Execution
