src/ReactorModel/Execution/State.lean
@@ -28,6 +28,9 @@ structure Allows (s : State) (rcn : ID) : Prop where
   deps : s.rtr.dependencies rcn ⊆ s.progress
   unprocessed : rcn ∉ s.progress
 
+theorem Allows.acyclic {s : State} (a : s.Allows rcn) : ¬(rcn <[s.rtr] rcn) :=
+  fun hc => absurd (a.deps hc) a.unprocessed
+
 def input (s : State) (rcn : s.rtr.Valid .rcn) : Reaction.Input where
   ports k := s.rtr[.prt k].restrict { i | .port k i ∈ rcn.obj.deps .in }
   acts    := s.rtr[.act].restrict { i | .action i ∈ rcn.obj.deps .in } |>.filterMap (·.lookup s.tag)
@@ -36,6 +39,10 @@ def input (s : State) (rcn : s.rtr.Valid .rcn) : Reaction.Input where
   
 def Triggers (s : State) (rcn : s.rtr.Valid .rcn) : Prop :=
   rcn.obj.TriggersOn (s.input rcn)
+
+theorem Triggers.progress_agnostic 
+    (h : Triggers s₁ ⟨i, h₁⟩) (hr : s₁.rtr = s₂.rtr) (ht : s₁.tag = s₂.tag) : Triggers s₂ ⟨i, h₂⟩ :=
+  sorry
 
 def exec (s : State) (rcn : s.rtr.Valid .rcn) : State :=
   { s with rtr := s.rtr.apply' $ rcn.obj (s.input rcn) }  
